theories/common/math.v
@@ -1,0 +1,17 @@
+From heap_lang Require Import
+  prelude.
+
+Section Z.
+  #[local] Open Scope Z_scope.
+
+  Lemma Z_rem_mod x y :
+    0 ≤ x →
+    0 ≤ y →
+    x `rem` y = x `mod` y.
+  Proof.
+    intros Hx Hy.
+    destruct (decide (y = 0)) as [-> | Hy'].
+    - rewrite Z.mod_0_r_ext // Z.rem_0_r_ext //.
+    - rewrite Z.rem_mod_nonneg //. lia.
+  Qed.
+End Z.
